theories/reg_addr.v
@@ -1,3 +1,4 @@
+(* this file contains basic definitions and lemmas about registers and addresses *)
 From Coq Require Import ssreflect Eqdep_dec ZArith.
 From HypVeri Require Import machine monad.
 From stdpp Require Import fin_maps list countable fin vector.
@@ -12,6 +13,7 @@ Ltac solveRegCount :=
   unfold reg_count;
   lia.
 
+(* we define these because they are frequently used *)
 Program Definition W0 : Word := (finz.FinZ 0 _ _).
 Solve Obligations with solveWordSize.
 
@@ -30,245 +32,265 @@ Solve Obligations with solveRegCount.
 Program Definition R2 :reg_name := (R 2 _).
 Solve Obligations with solveRegCount.
 
+Definition list_of_W0: list Word:=
+  map (λ _, W0) (seq 0 (Z.to_nat page_size)).
 
-  (** predicates and lemmas for checking if addresses/regions are in a page *)
-  Definition addr_in_page (a: Addr ) (p:PID):=
-    ((of_pid p) <=? a)%f ∧ (a <=? ((of_pid p) ^+ (page_size -1 )))%f.
-
-  Definition seq_in_page (b :Addr) (l: nat) (p:PID) :=
-    ((of_pid p) <=? b)%Z ∧ is_Some (b + (Z.of_nat l))%f ∧ ((b ^+ (Z.of_nat l))%f <=? ((of_pid p) ^+ (page_size-1))%f)%Z.
+Lemma length_list_of_W0 : length (list_of_W0) = (Z.to_nat page_size).
+Proof.
+  rewrite /list_of_W0 map_length seq_length //.
+Qed.
 
 
-  Lemma last_addr_in_bound (p:PID):
-    is_Some ((of_pid p) + (page_size -1)%Z)%f.
-    Proof.
-      destruct p.
-      destruct z.
-      simplify_eq /=.
-      assert (Hy : exists y, (y * page_size = word_size)%Z).
-      exists 2000%Z.
-      unfold page_size, word_size.
+(* an address is in the range of the page with PID p *)
+Definition addr_in_page (a: Addr ) (p:PID):=
+  ((of_pid p) <=? a)%f ∧ (a <=? ((of_pid p) ^+ (page_size -1 )))%f.
+
+(* a sequence of addresses is in the range of the page with PID p *)
+Definition seq_in_page (b :Addr) (l: nat) (p:PID) :=
+  (* the starting address b is greater than the base addr of the page *)
+  ((of_pid p) <=? b)%Z
+  (* the ending address doesn't excess the boundary of address space *)
+  ∧ is_Some (b + (Z.of_nat l))%f
+  (* the ending address is less than or equal to the last address of the page *)
+  ∧ ((b ^+ (Z.of_nat l))%f <=? ((of_pid p) ^+ (page_size-1))%f)%Z.
+
+(* we can always get the last address of a page *)
+Lemma last_addr_in_bound (p:PID):
+  is_Some ((of_pid p) + (page_size -1)%Z)%f.
+Proof.
+  destruct p.
+  destruct z.
+  simplify_eq /=.
+  assert (Hy : exists y, (y * page_size = word_size)%Z).
+  exists 2000%Z.
+  unfold page_size, word_size.
+  lia.
+  destruct Hy.
+  assert (Hlt: (z + page_size -1 < word_size)%Z).
+  {
+    apply Z.ltb_lt in finz_lt.
+    apply Z.leb_le in finz_nonneg.
+    assert (Hlt': (z  < word_size - page_size + 1 )%Z).
+    {
+      destruct (decide (z  < word_size - page_size + 1)%Z).
       lia.
-      destruct Hy.
-      assert (Hlt: (z + page_size -1 < word_size)%Z).
-      {
-       apply Z.ltb_lt in finz_lt.
-       apply Z.leb_le in finz_nonneg.
-       assert (Hlt': (z  < word_size - page_size + 1 )%Z).
-       {
-         destruct (decide (z  < word_size - page_size + 1)%Z).
-         lia.
-         assert(H': ( (x -1 ) * page_size < z )%Z).
-         lia.
-         apply Z.eqb_eq in align.
-         apply Z.rem_divide in align;[|unfold page_size;lia].
-         destruct align.
-         subst z.
-         rewrite -H in finz_lt.
-         apply Zmult_gt_0_lt_reg_r in finz_lt;[|unfold page_size;lia].
-         apply Zmult_gt_0_lt_reg_r in H';[|unfold page_size;lia].
-         lia.
-       }
-       lia.
-       }
-      unfold finz.incr.
-      simpl.
-      destruct (Z_lt_dec (z + (page_size - 1))%Z word_size).
-      destruct (Z_le_dec 0%Z (z + (page_size - 1))%Z).
-      eauto.
-      exfalso.
-      apply n.
-      unfold page_size.
+      assert(H': ( (x -1 ) * page_size < z )%Z).
       lia.
-      exfalso.
-      apply n.
-      lia.
-  Qed.
-
-  Lemma incr_default_incr{fb} (f1 f2: finz.finz fb) z : (f1 + z)%f = Some f2 ->
-                                    (f1 ^+ z)%f = f2.
-  Proof.
-    intro.
-    solve_finz.
-  Qed.
-
-  Lemma finz_incr_z_plus{b} (f1 f2 : (finz.finz b)) z : (f1 + z)%f = Some f2 <->
-                                                        (f1 + z)%Z = (finz.to_z f2).
-  Proof.
-    split;solve_finz.
-  Qed.
-
-  Lemma finz_incr_z_plus'{b} (f1 : (finz.finz b)) z : (f1 + z)%f = None <->
-                                                      (b <= (f1 + z))%Z ∨ ((f1 +z) < 0)%Z .
-  Proof.
-    split; solve_finz.
-  Qed.
-
-  Lemma finz_plus_Z_lt{b} (f: (finz.finz b)) z1 z2:
-    (is_Some (f + z1)%f) -> (is_Some (f + z2)%f) ->
-  ((f ^+ z1)%f < (f ^+ z2)%f)%Z -> (z1 < z2)%Z.
-    Proof.
-      intros H1 H2 Hlt.
-      destruct H1 as [f1 H1].
-      destruct H2 as [f2 H2].
-      rewrite (incr_default_incr f f1 z1) in Hlt;eauto.
-      rewrite (incr_default_incr f f2 z2) in Hlt;eauto.
-      solve_finz.
-    Qed.
-
-  Lemma finz_plus_Z_le{b} (f: (finz.finz b)) z1 z2:
-    (is_Some (f + z1)%f) -> (is_Some (f + z2)%f) ->
-  ((f ^+ z1)%f <= (f ^+ z2)%f)%Z -> (z1 <= z2)%Z.
-    Proof.
-      intros H1 H2 Hlt.
-      destruct H1 as [f1 H1].
-      destruct H2 as [f2 H2].
-      rewrite (incr_default_incr f f1 z1) in Hlt;eauto.
-      rewrite (incr_default_incr f f2 z2) in Hlt;eauto.
-      solve_finz.
-    Qed.
-
-
-  Lemma to_pid_aligned_in_page (a:Addr) (p:PID) :
-    addr_in_page a p -> (to_pid_aligned a ) = p.
-    Proof.
-      intro.
-      unfold to_pid_aligned.
-      unfold addr_in_page in H.
-      destruct H.
-      pose proof (last_addr_in_bound p).
-      destruct H1.
-      rewrite (incr_default_incr (of_pid p) x (page_size -1)%Z) in H0;eauto.
-      destruct p.
-      destruct z.
-      f_equal /=.
-      assert (Heq : z = (page_size * (a / page_size))%Z).
-      {
-        destruct a.
-        simplify_eq /=.
-        unfold finz.leb in H.
-        simpl in H.
-        unfold finz.ltb in H0.
-        simpl in H0.
-        apply Is_true_eq_true in H, H0.
-        apply Z.leb_le in H.
-        apply Z.leb_le in H0.
-        apply finz_incr_z_plus in H1.
-        simpl in H1.
-        rewrite -H1 in H0.
-        simpl in H0.
-        apply Z.eqb_eq in align.
-        apply Z.rem_divide in align;[|unfold page_size;lia].
-        destruct align.
-        subst z.
-       apply (fast_Zmult_comm page_size x0) in H.
-        apply Z.quot_le_lower_bound in H;[|unfold page_size;lia].
-       assert (H0': (z0 < page_size* (x0+1) )%Z).
-       lia.
-       apply Z.quot_lt_upper_bound in H0';[|lia|unfold page_size;lia].
-       assert (Heq: (z0 `quot` page_size = x0)%Z).
-       lia.
-       rewrite Z.quot_div_nonneg in Heq;[lia|unfold page_size;lia| ].
-       solve_finz.
-      }
+      apply Z.eqb_eq in align.
+      apply Z.rem_divide in align;[|unfold page_size;lia].
+      destruct align.
       subst z.
-      remember (machine.to_pid_aligned_obligation_3 a) as Ha'.
-      simpl in Ha'.
-      assert (Heqiv : Ha' = align).
-      apply eq_proofs_unicity; decide equality; decide equality.
-      rewrite Heqiv.
-      remember (machine.to_pid_aligned_obligation_1 a) as Ha''.
-      simpl in  Ha''.
-      remember (machine.to_pid_aligned_obligation_2 a) as Ha'''.
-      simpl in  Ha'''.
-      assert (Heqiv' : Ha'' = finz_lt).
-      apply eq_proofs_unicity; decide equality; decide equality.
-      rewrite Heqiv'.
-      assert (Heqiv'' : Ha''' = finz_nonneg).
-      apply eq_proofs_unicity; decide equality; decide equality.
-      rewrite Heqiv'' // .
+      rewrite -H in finz_lt.
+      apply Zmult_gt_0_lt_reg_r in finz_lt;[|unfold page_size;lia].
+      apply Zmult_gt_0_lt_reg_r in H';[|unfold page_size;lia].
+      lia.
+    }
+    lia.
+  }
+  unfold finz.incr.
+  simpl.
+  destruct (Z_lt_dec (z + (page_size - 1))%Z word_size).
+  destruct (Z_le_dec 0%Z (z + (page_size - 1))%Z).
+  eauto.
+  exfalso.
+  apply n.
+  unfold page_size.
+  lia.
+  exfalso.
+  apply n.
+  lia.
 Qed.
 
-    Lemma finz_seq_notin2{b} (f f' : finz.finz b) n :
-      (f' ^+ ((Z.of_nat n)-1) < f)%f -> f ∉ finz.seq f' n.
-    Proof.
-      revert f f'. induction n; cbn.
-      { intros. inversion 1. }
-      { intros. apply not_elem_of_cons. split. solve_finz. eapply IHn. solve_finz. }
-     Qed.
-
-    Lemma finz_seq_in2{b} (f f' : finz.finz b) n :
-     f ∈ finz.seq f' n ->  (f <= f' ^+ ((Z.of_nat n)-1))%f.
-    Proof.
-      revert f f'. induction n; cbn.
-      { intros. inversion H. }
-      { intros. apply  elem_of_cons in H.
-        destruct H.
-        solve_finz.
-        eapply IHn in H. solve_finz. }
-     Qed.
-
-    Definition seq_in_page_forall (b: Addr) (l:nat) (p:PID) :
-    seq_in_page b l p -> Forall  (λ a, addr_in_page a p) (finz.seq b l).
-    Proof.
-      intros.
-      apply Forall_forall.
-      intros a H0.
-      unfold addr_in_page.
-      destruct H.
-      split.
-      - unfold finz.leb.
-        unfold Is_true.
-        destruct (decide (b <= a)%f).
-        unfold Is_true in H.
-        assert (Hap: ((of_pid p) <= a)%Z).
-        destruct ((((of_pid p) <=? b))%Z) eqn:Heqn.
-        apply Z.leb_le in Heqn.
-        solve_finz.
-        congruence.
-        apply Z.leb_le in Hap.
-        rewrite Hap //=.
-        exfalso.
-        assert (Hlt: (a < b )%f).
-        solve_finz.
-        apply (finz_seq_notin _ _ _ l )in Hlt.
-        contradiction.
-      - destruct l.
-        inversion H0.
-        destruct H1.
-        destruct H1.
-        rewrite (incr_default_incr b x _ ) in H2;eauto.
-        pose proof (last_addr_in_bound p).
-        destruct H3.
-        rewrite (incr_default_incr (of_pid p) x0 _ ) in H2;eauto.
-        rewrite (incr_default_incr (of_pid p) x0 _ );eauto.
-        apply  finz_incr_z_plus in H3.
-        apply finz_seq_in2 in H0.
-        apply  finz_incr_z_plus in H1.
-        assert (H1': (b + (Z.of_nat l))%Z = (x-1)%Z ). by lia.
-        assert(Hl : ((Z.of_nat (S l) - 1)%Z = (Z.of_nat l))%Z).  by lia.
-        rewrite Hl  in H0 H1.
-        rewrite -H3 in H2.
-        rewrite -H1 in H2.
-        unfold finz.leb.
-        rewrite -H3.
-        assert (H0': (a <= b + (Z.of_nat l))%Z).
-        solve_finz.
-        rewrite -H1 in H1'.
-        destruct (decide (a <= (of_pid p) + (page_size - 1)))%Z.
-        apply Z.leb_le in l0.
-        solve_finz.
-        exfalso.
-        destruct ((b + Z.of_nat (S l) <=? (of_pid p) + (page_size - 1))%Z) eqn:Heqn.
-        apply Z.leb_le in Heqn.
-        lia.
-        contradiction.
+(* complementing lemmas for finz *)
+Lemma incr_default_incr{fb} (f1 f2: finz.finz fb) z :
+  (f1 + z)%f = Some f2 -> (f1 ^+ z)%f = f2.
+Proof.
+  intro.
+  solve_finz.
 Qed.
 
+Lemma finz_incr_z_plus{b} (f1 f2 : (finz.finz b)) z :
+  (f1 + z)%f = Some f2 <-> (f1 + z)%Z = (finz.to_z f2).
+Proof.
+  split;solve_finz.
+Qed.
+
+Lemma finz_incr_z_plus'{b} (f1 : (finz.finz b)) z :
+  (f1 + z)%f = None <-> (b <= (f1 + z))%Z ∨ ((f1 +z) < 0)%Z .
+Proof.
+  split; solve_finz.
+Qed.
+
+Lemma finz_plus_Z_lt{b} (f: (finz.finz b)) z1 z2:
+  (is_Some (f + z1)%f) -> (is_Some (f + z2)%f) ->
+  ((f ^+ z1)%f < (f ^+ z2)%f)%Z -> (z1 < z2)%Z.
+Proof.
+  intros H1 H2 Hlt.
+  destruct H1 as [f1 H1].
+  destruct H2 as [f2 H2].
+  rewrite (incr_default_incr f f1 z1) in Hlt;eauto.
+  rewrite (incr_default_incr f f2 z2) in Hlt;eauto.
+  solve_finz.
+Qed.
+
+Lemma finz_plus_Z_le{b} (f: (finz.finz b)) z1 z2:
+  (is_Some (f + z1)%f) ->
+  (is_Some (f + z2)%f) ->
+  ((f ^+ z1)%f <= (f ^+ z2)%f)%Z ->
+  (z1 <= z2)%Z.
+Proof.
+  intros H1 H2 Hlt.
+  destruct H1 as [f1 H1].
+  destruct H2 as [f2 H2].
+  rewrite (incr_default_incr f f1 z1) in Hlt;eauto.
+  rewrite (incr_default_incr f f2 z2) in Hlt;eauto.
+  solve_finz.
+Qed.
+
+(*  relation between to_pid_aligned and addr_in_page,
+ TODO: prove the opposite direction (not sure if is useful) *)
+Lemma to_pid_aligned_in_page (a:Addr) (p:PID) :
+  addr_in_page a p -> (to_pid_aligned a ) = p.
+Proof.
+  intro.
+  unfold to_pid_aligned.
+  unfold addr_in_page in H.
+  destruct H.
+  pose proof (last_addr_in_bound p).
+  destruct H1.
+  rewrite (incr_default_incr (of_pid p) x (page_size -1)%Z) in H0;eauto.
+  destruct p.
+  destruct z.
+  f_equal /=.
+  assert (Heq : z = (page_size * (a / page_size))%Z).
+  {
+    destruct a.
+    simplify_eq /=.
+    unfold finz.leb in H.
+    simpl in H.
+    unfold finz.ltb in H0.
+    simpl in H0.
+    apply Is_true_eq_true in H, H0.
+    apply Z.leb_le in H.
+    apply Z.leb_le in H0.
+    apply finz_incr_z_plus in H1.
+    simpl in H1.
+    rewrite -H1 in H0.
+    simpl in H0.
+    apply Z.eqb_eq in align.
+    apply Z.rem_divide in align;[|unfold page_size;lia].
+    destruct align.
+    subst z.
+    apply (fast_Zmult_comm page_size x0) in H.
+    apply Z.quot_le_lower_bound in H;[|unfold page_size;lia].
+    assert (H0': (z0 < page_size* (x0+1) )%Z).
+    lia.
+    apply Z.quot_lt_upper_bound in H0';[|lia|unfold page_size;lia].
+    assert (Heq: (z0 `quot` page_size = x0)%Z).
+    lia.
+    rewrite Z.quot_div_nonneg in Heq;[lia|unfold page_size;lia| ].
+    solve_finz.
+  }
+  subst z.
+  remember (machine.to_pid_aligned_obligation_3 a) as Ha'.
+  simpl in Ha'.
+  assert (Heqiv : Ha' = align).
+  apply eq_proofs_unicity; decide equality; decide equality.
+  rewrite Heqiv.
+  remember (machine.to_pid_aligned_obligation_1 a) as Ha''.
+  simpl in  Ha''.
+  remember (machine.to_pid_aligned_obligation_2 a) as Ha'''.
+  simpl in  Ha'''.
+  assert (Heqiv' : Ha'' = finz_lt).
+  apply eq_proofs_unicity; decide equality; decide equality.
+  rewrite Heqiv'.
+  assert (Heqiv'' : Ha''' = finz_nonneg).
+  apply eq_proofs_unicity; decide equality; decide equality.
+  rewrite Heqiv'' // .
+Qed.
+
+(* complementing lemmas for finz.seq *)
+Lemma finz_seq_notin2{b} (f f' : finz.finz b) n :
+  (f' ^+ ((Z.of_nat n)-1) < f)%f -> f ∉ finz.seq f' n.
+Proof.
+  revert f f'. induction n; cbn.
+  { intros. inversion 1. }
+  { intros. apply not_elem_of_cons. split. solve_finz. eapply IHn. solve_finz. }
+Qed.
+
+Lemma finz_seq_in2{b} (f f' : finz.finz b) n :
+  f ∈ finz.seq f' n ->  (f <= f' ^+ ((Z.of_nat n)-1))%f.
+Proof.
+  revert f f'. induction n; cbn.
+  { intros. inversion H. }
+  { intros. apply  elem_of_cons in H.
+    destruct H.
+    solve_finz.
+    eapply IHn in H. solve_finz. }
+Qed.
+
+(* if the sequcence is included in a page,
+then every address in the sequcence is in the page *)
+Definition seq_in_page_forall (b: Addr) (l:nat) (p:PID) :
+  seq_in_page b l p -> Forall  (λ a, addr_in_page a p) (finz.seq b l).
+Proof.
+  intros.
+  apply Forall_forall.
+  intros a H0.
+  unfold addr_in_page.
+  destruct H.
+  split.
+  - unfold finz.leb.
+    unfold Is_true.
+    destruct (decide (b <= a)%f).
+    unfold Is_true in H.
+    assert (Hap: ((of_pid p) <= a)%Z).
+    destruct ((((of_pid p) <=? b))%Z) eqn:Heqn.
+    apply Z.leb_le in Heqn.
+    solve_finz.
+    congruence.
+    apply Z.leb_le in Hap.
+    rewrite Hap //=.
+    exfalso.
+    assert (Hlt: (a < b )%f).
+    solve_finz.
+    apply (finz_seq_notin _ _ _ l )in Hlt.
+    contradiction.
+  - destruct l.
+    inversion H0.
+    destruct H1.
+    destruct H1.
+    rewrite (incr_default_incr b x _ ) in H2;eauto.
+    pose proof (last_addr_in_bound p).
+    destruct H3.
+    rewrite (incr_default_incr (of_pid p) x0 _ ) in H2;eauto.
+    rewrite (incr_default_incr (of_pid p) x0 _ );eauto.
+    apply  finz_incr_z_plus in H3.
+    apply finz_seq_in2 in H0.
+    apply  finz_incr_z_plus in H1.
+    assert (H1': (b + (Z.of_nat l))%Z = (x-1)%Z ). by lia.
+    assert(Hl : ((Z.of_nat (S l) - 1)%Z = (Z.of_nat l))%Z).  by lia.
+    rewrite Hl  in H0 H1.
+    rewrite -H3 in H2.
+    rewrite -H1 in H2.
+    unfold finz.leb.
+    rewrite -H3.
+    assert (H0': (a <= b + (Z.of_nat l))%Z).
+    solve_finz.
+    rewrite -H1 in H1'.
+    destruct (decide (a <= (of_pid p) + (page_size - 1)))%Z.
+    apply Z.leb_le in l0.
+    solve_finz.
+    exfalso.
+    destruct ((b + Z.of_nat (S l) <=? (of_pid p) + (page_size - 1))%Z) eqn:Heqn.
+    apply Z.leb_le in Heqn.
+    lia.
+    contradiction.
+Qed.
 
 Lemma finz_seq_lookup'{b} (f0 fi:(finz.finz b)) (i n : nat) :
-   is_Some(f0 + (Z.of_nat n))%f ->
-   finz.seq f0 n !! i = Some fi ->
+  is_Some(f0 + (Z.of_nat n))%f ->
+  finz.seq f0 n !! i = Some fi ->
   i < n ∧ (f0 + (Z.of_nat i))%f = Some fi.
 Proof using.
   revert i fi f0. induction n.
@@ -282,3 +304,8 @@ Proof using.
       split.
       lia. rewrite -H0. solve_finz. solve_finz. } }
 Qed.
+
+Definition addr_of_page (p: PID) := (finz.seq (of_pid p) (Z.to_nat page_size)).
+
+(* an alternative definition, not sure which is better *)
+(* Definition addr_of_page' (p: PID) := map (λ off, ((of_pid p) + off)%f) (seqZ 0%Z page_size). *)
