theories/rules/donate.v
@@ -215,4 +215,234 @@ Proof.
      by iFrame.
 Qed.
 
+
+Lemma hvc_donate_z {instr i wi r2 pi ptx sown q sacc sexcl des sh} {l :Word} {spsd: gset PID}
+      ai r0 r1 j (psd: list PID):
+  (* the current instruction is hvc *)
+  instr = Hvc ->
+  (* the decoding of wi is correct *)
+  decode_instruction wi = Some(instr) ->
+  (* the instruction is in page pi *)
+  addr_in_page ai pi ->
+  (* the decoding of R0 is FFA_DONATE *)
+  decode_hvc_func r0 = Some(Donate) ->
+  (* caller is not the receiver *)
+  i ≠ j ->
+  (* l is the number of to-be-donated pages *)
+  (finz.to_z l) = (Z.of_nat (length psd)) ->
+  (* the descriptor, in list Word *)
+  des = serialized_transaction_descriptor i j W1 l psd W0 ->
+  (* the whole descriptor resides in the TX page *)
+  seq_in_page (of_pid ptx) (length des) ptx ->
+  (* r1 equals the length of the descriptor *)
+  (finz.to_z r1) = (Z.of_nat (length des)) ->
+  (* spsd is the gset of all to-be-donated pages *)
+  spsd = (list_to_set psd) ->
+  (* pi and pages in spsd are accessible for VM i *)
+  {[pi]} ∪ spsd ⊆ sacc ->
+  (* VM i owns pages in spsd *)
+  spsd ⊆ sown ->
+  (* pages in spsed are exclusive to VM i *)
+  spsd ⊆ sexcl ->
+  (* there are at least one free handles in the hpool *)
+  sh ≠ ∅ ->
+  {SS{{ ▷(PC @@ i ->r ai) ∗ ▷ ai ->a wi
+  ∗ ▷ O@i:={q}[sown] ∗ ▷ A@i:={1}[sacc] ∗ ▷ E@i:={1}[sexcl]
+  ∗ ▷ (R0 @@ i ->r r0) ∗ ▷ (R1 @@ i ->r r1) ∗ ▷(R2 @@i ->r r2) ∗  ▷ TX@ i := ptx
+  ∗ ▷ mem_region des ptx ∗ ▷ ([∗ list] p ∈ psd, mem_page p [])
+  ∗ ▷ hp{ 1 }[ sh ] }}}
+   ExecI @ i {{{ RET ExecI ; PC @@ i ->r (ai ^+ 1)%f ∗ ai ->a wi
+  ∗ O@i:={q}[sown] ∗ A@i:={1}[sacc∖spsd] ∗ E@i:={1}[sexcl∖spsd]
+  ∗ R0 @@ i ->r (encode_hvc_ret_code Succ) ∗ R1 @@ i ->r r1  ∗ TX@ i := ptx
+  ∗ ∃(wh: Word), ( ⌜ wh ∈ sh ⌝ ∗ R2 @@ i ->r wh ∗ wh ->t{1}(i,W0, j , psd,Donation)
+  ∗ wh ->re false  ∗ hp{1}[ (sh∖{[wh]})] )
+  ∗ mem_region des ptx ∗ ([∗ list] p ∈ psd, mem_page p list_of_W0)}}}.
+Proof.
+  iIntros (Hinstr Hdecodei Hini Hdecodef Hneq Hlenpsd Hdesc Hindesc Hlenr1 Hspsd Hsacc Hsown Hsexcl Hshne Φ ).
+  iIntros "(>PC & >Hai & >Hown & >Hacc & >Hexcl & >R0 & >R1 & >R2 & >TX & >Hadesc & >Hpgs & >Hhp ) HΦ".
+  iApply (sswp_lift_atomic_step ExecI);[done|].
+  iIntros (σ1) "%Hsche Hσ".
+  inversion Hsche as [ Hcureq ]; clear Hsche.
+  apply fin_to_nat_inj in Hcureq.
+  iModIntro.
+  iDestruct "Hσ" as "(Hcur & Hσmem & Hσreg & Hσtx & ? & Hσowned & Hσaccess & Hσexcl & Htrans & Hσhp & %Hdisj & Hrcv)".
+  (* valid regs *)
+  iDestruct ((gen_reg_valid4 σ1 i PC ai R0 r0 R1 r1 R2 r2 Hcureq ) with "Hσreg PC R0 R1 R2 ")
+    as "[%HPC [%HR0 [%HR1 %HR2]]]";eauto.
+  (* valid pt *)
+  iDestruct ((gen_access_valid_addr_elem ai sacc) with "Hσaccess Hacc") as %Haccai;eauto.
+  { rewrite (to_pid_aligned_in_page _ pi);eauto. set_solver. }
+  iDestruct ((gen_access_valid_lookup_Set _ _ _ sacc) with "Hσaccess Hacc") as %Hacc;eauto.
+  iDestruct ((gen_own_valid_Set sown) with "Hσowned Hown") as %Hown;eauto.
+  iDestruct ((gen_excl_valid_Set sexcl) with "Hσexcl Hexcl") as %Hexcl;eauto.
+  iDestruct ((gen_excl_valid_lookup_Set _ _ _ sexcl) with "Hσexcl Hexcl") as %Hexcl';eauto.
+  (* valid mem *)
+  iDestruct (gen_mem_valid σ1 ai wi with "Hσmem Hai") as %Hai.
+  unfold mem_region.
+  iDestruct (gen_mem_valid_SepL_pure _ des with "Hσmem Hadesc") as %Hadesc.
+  { apply finz_seq_NoDup. destruct Hindesc as [? [HisSome ?]]. done. }
+  (* valid tx *)
+  iDestruct (gen_tx_valid with "TX Hσtx") as %Htx.
+  (* valid hpool *)
+  iDestruct (gen_hpool_valid1 with "Hhp Hσhp") as %Hhp.
+  iSplit.
+  - (* reducible *)
+    iPureIntro.
+    apply (reducible_normal i instr ai wi);eauto.
+  - (* step *)
+    iModIntro.
+    iIntros (m2 σ2) "%HstepP".
+    apply (step_ExecI_normal i instr ai wi) in HstepP;eauto.
+    remember (exec instr σ1) as c2 eqn:Heqc2.
+    assert (Hlendesclt :((Z.of_nat (length des)) <= (page_size-1))%Z).
+    {  destruct Hindesc as [? [HisSome Hltpagesize]]. apply (finz_plus_Z_le (of_pid ptx));eauto.
+       apply last_addr_in_bound.  apply Z.leb_le. destruct (((ptx ^+ length des)%f <=? (ptx ^+ (page_size - 1))%f)%Z). done. contradiction. }
+    rewrite /exec Hinstr /hvc HR0 Hdecodef /mem_send //= HR1 /= in Heqc2.
+    destruct (page_size <? r1)%Z eqn:Heqn;[lia|clear Heqn].
+    rewrite Hcureq /get_tx_pid_global Htx (@transaction_descriptor_valid i j W1 l psd σ1 des) /= in Heqc2;eauto.
+    assert (Hcheck : (i =? i) = true).
+    { by apply   <- Nat.eqb_eq. }
+    rewrite Hcureq Hcheck /= in Heqc2;clear Hcheck.
+    assert (Hcheck:  negb (i =? j) = true).
+       {apply negb_true_iff. apply  <- Nat.eqb_neq. intro. apply Hneq. by apply fin_to_nat_inj.  }
+    rewrite Hcheck /= in Heqc2;clear Hcheck.
+    destruct (forallb (λ v' : PID, check_perm_page σ1 i v' (Owned, ExclusiveAccess))
+                                    psd) eqn:HCheck.
+    2: {
+      apply not_true_iff_false in HCheck.
+      exfalso.
+      apply HCheck.
+      apply forallb_forall.
+      intros.
+      unfold check_perm_page.
+      apply elem_of_list_In in H.
+      apply (elem_of_list_to_set (C:= gset PID)) in H.
+      rewrite <- Hspsd in H.
+      assert (HxInown: x ∈ sown). { set_solver. }
+      assert (HxInexcl: x ∈ sexcl). { set_solver. }
+      pose proof (Hown x HxInown) as Hxown .
+      simpl in Hxown.
+      destruct Hxown as [perm [HSomeperm Hisowned]].
+      rewrite /check_ownership_page  HSomeperm /=.
+      destruct (decide (Owned = perm)). simpl.
+      2: { exfalso. apply n. destruct perm;eauto. rewrite /is_owned //.  }
+      pose proof (Hexcl x HxInexcl) as Hxexcl.
+      simpl in Hxexcl.
+      destruct Hxexcl as [perm' [HSomeperm' Hisexcl]].
+      rewrite /check_access_page HSomeperm'.
+      destruct (decide (ExclusiveAccess = perm')). done.
+      exfalso. apply n. destruct perm';eauto; rewrite /is_exclusive //.
+    }
+    rewrite /new_transaction /fresh_handle in Heqc2.
+    destruct (elements sh) as [| h fhs] eqn:Hfhs .
+    { exfalso. rewrite -elements_empty in Hfhs.  apply Hshne. apply set_eq.
+     intro. rewrite -elem_of_elements Hfhs elem_of_elements.   split;intro;set_solver. }
+    rewrite -Hhp //=  in Heqc2.
+    destruct HstepP;subst m2 σ2; subst c2; simpl.
+    rewrite /gen_vm_interp /update_incr_PC /update_reg.
+    (* unchanged part *)
+    rewrite_reg_all.
+    rewrite update_access_batch_preserve_current_vm
+            zero_pages_preserve_current_vm insert_transaction_preserve_current_vm.
+    rewrite_reg_all.
+    rewrite_access_all.
+    rewrite_mem_all.
+    rewrite_trans_all.
+    iFrame.
+    (* update regs *)
+     rewrite -> (update_offset_PC_update_PC1 _ i ai 1);eauto.
+     rewrite !update_reg_global_update_reg ?update_access_batch_preserve_regs
+             ?zero_pages_preserve_reg ?insert_transaction_preserve_regs;try solve_reg_lookup.
+     2 : {
+        exists r2.
+        rewrite lookup_insert_ne.
+        solve_reg_lookup.
+        done.
+     }
+     2 : { rewrite !update_reg_global_preserve_current_vm  update_access_batch_preserve_current_vm
+            zero_pages_preserve_current_vm insert_transaction_preserve_current_vm //. }
+     2 : {
+        rewrite !update_reg_global_update_reg.
+        rewrite ?update_access_batch_preserve_regs
+                ?zero_pages_preserve_reg
+                ?insert_transaction_preserve_regs;try solve_reg_lookup.
+        rewrite !lookup_insert_ne;[solve_reg_lookup|done|done].
+        rewrite ?update_access_batch_preserve_regs
+                ?zero_pages_preserve_reg
+                ?insert_transaction_preserve_regs;try solve_reg_lookup.
+        rewrite ?update_access_batch_preserve_regs
+                ?zero_pages_preserve_reg
+                ?insert_transaction_preserve_regs.
+        exists r2.
+        rewrite lookup_insert_ne;[solve_reg_lookup|done].
+        rewrite ?update_access_batch_preserve_regs
+                ?zero_pages_preserve_reg
+                ?insert_transaction_preserve_regs.
+        solve_reg_lookup.
+     }
+     iDestruct ((gen_reg_update3_global PC i (ai ^+ 1)%f R2 i h R0 i (encode_hvc_ret_code Succ) ) with "Hσreg PC R2 R0") as ">[Hσreg [PC [R2 R0]]]";eauto.
+     rewrite Hcureq.
+     iFrame.
+     (* TODO: update memory *)
+     (* don't know how to express it *)
+     (* update page table *)
+     rewrite (@update_access_batch_update_access_diff _ i sacc spsd psd);eauto.
+     rewrite ?zero_pages_preserve_current_vm ?insert_transaction_preserve_current_vm.
+     iDestruct ((gen_access_update_diff spsd) with "Hacc Hσaccess") as ">[Hσaccess Hacc]";eauto.
+     set_solver.
+     rewrite Hcureq.
+     rewrite zero_pages_preserve_access
+             insert_transaction_preserve_access.
+     rewrite update_access_batch_preserve_ownerships
+             zero_pages_preserve_owned
+             insert_transaction_preserve_owned.
+     rewrite (@update_access_batch_update_excl_diff _ i sexcl spsd psd);eauto.
+     rewrite ?zero_pages_preserve_current_vm ?insert_transaction_preserve_current_vm.
+     rewrite zero_pages_preserve_excl
+             insert_transaction_preserve_excl.
+     iDestruct ((gen_excl_update_diff spsd) with "Hexcl Hσexcl") as ">[Hσexcl Hexcl]";eauto.
+     rewrite Hcureq.
+     iFrame.
+     (* update transactions *)
+     rewrite insert_transaction_update_trans /=.
+     rewrite insert_transaction_update_hpool /=.
+     rewrite insert_transaction_update_retri /=.
+     assert (HhInfhs: h ∈ (get_transactions σ1).2). {
+        rewrite /get_fresh_handles in Hhp.
+        apply elem_of_elements.
+        rewrite -Hhp.
+        apply <- (elem_of_cons fhs h h).
+        left;done.
+     }
+     iDestruct ((gen_trans_update_insert h i W1 j psd Donation) with "Htrans") as ">[Hσtrans Htran]".
+     { apply not_elem_of_dom.
+       rewrite get_trans_gmap_preserve_dom.
+       set_solver.
+     }
+     assert (HhIn: h ∈ sh).
+      { apply elem_of_elements.
+       rewrite Hfhs.
+       apply <- (elem_of_cons fhs h h).
+       left;done.
+     }
+     iDestruct ((gen_hpool_update_diff h HhIn) with "Hhp Hσhp") as ">[Hσhp Hhp]".
+     iDestruct ((gen_retri_update_insert h) with "Hrcv") as ">[Hσrtrv Hrtrv]".
+     { apply not_elem_of_dom.
+       rewrite get_retri_gmap_preserve_dom.
+       set_solver.
+     }
+     iFrame.
+     iModIntro.
+     iSplitR.
+     iPureIntro.
+     set_solver.
+     iApply "HΦ".
+     iFrame.
+     iExists h.
+     by iFrame.
+Qed.
+
+
+
+
 End donate.
